NuInstructions.thy
@@ -71,13 +71,13 @@ subsubsection \<open>let & local_value\<close>
 
 definition op_let :: " ('v::lrep \<Rightarrow> 's::stack \<longmapsto> 't::stack) \<Rightarrow> ('v \<times> 's \<longmapsto> 't)"
   where "op_let body = (\<lambda>(h,v,s). body v (h,s))"
-lemma op_let: " (\<And>p. p \<nuLinkL> A \<nuLinkR> a \<Longrightarrow> \<^bold>p\<^bold>r\<^bold>o\<^bold>c body p \<blangle> X \<longmapsto> X' \<brangle>) \<Longrightarrow>
-   \<^bold>p\<^bold>r\<^bold>o\<^bold>c op_let body \<blangle> X\<heavy_comma>^ a \<tycolon> A \<longmapsto> X' \<brangle>"
+lemma op_let: " (\<And>p. p \<nuLinkL> A \<nuLinkR> a \<Longrightarrow> \<^bold>p\<^bold>r\<^bold>o\<^bold>c body p \<blangle> S\<heavy_comma> \<^bold>h\<^bold>e\<^bold>a\<^bold>p H \<longmapsto> X' \<brangle>) \<Longrightarrow>
+   \<^bold>p\<^bold>r\<^bold>o\<^bold>c op_let body \<blangle> S\<heavy_comma> a \<tycolon> A\<heavy_comma> \<^bold>h\<^bold>e\<^bold>a\<^bold>p H \<longmapsto> X' \<brangle>"
   unfolding Procedure_def op_let_def by (auto simp add: nu_exps)
 
 definition op_local_value :: " 'v::lrep \<Rightarrow> 's::stack \<longmapsto> 'v \<times> 's "
   where "op_local_value v = (\<lambda>(h,s). Success (h,v,s))"
-lemma op_local_value: "v \<nuLinkL> A \<nuLinkR> a \<Longrightarrow> \<^bold>p\<^bold>r\<^bold>o\<^bold>c op_local_value v \<blangle> S\<heavy_comma> \<^bold>h\<^bold>e\<^bold>a\<^bold>p Nothing \<longmapsto> S\<heavy_comma> a \<tycolon> A\<heavy_comma> \<^bold>h\<^bold>e\<^bold>a\<^bold>p Nothing \<brangle>"
+lemma op_local_value: "v \<nuLinkL> A \<nuLinkR> a \<Longrightarrow> \<^bold>p\<^bold>r\<^bold>o\<^bold>c op_local_value v \<blangle> S\<heavy_comma> \<^bold>h\<^bold>e\<^bold>a\<^bold>p H \<longmapsto> S\<heavy_comma> a \<tycolon> A\<heavy_comma> \<^bold>h\<^bold>e\<^bold>a\<^bold>p H \<brangle>"
   unfolding Procedure_def op_local_value_def by (auto simp add: nu_exps)
 
 ML_file "library/local_value.ML"
@@ -169,15 +169,17 @@ lemma SemDoWhile_deterministic2: " SemDoWhile body s x \<Longrightarrow> The ( S
 definition DoWhile :: "('r \<longmapsto> 1 word \<times> 'r) \<Rightarrow> 'r \<longmapsto> 'r" where
   "DoWhile f s = (if (\<exists>y. SemDoWhile f s y) then The (SemDoWhile f s) else PartialCorrect)"
 
+declare Heap'_expn[simp del]
 lemma "__DoWhile___\<nu>app": "(\<forall>x. \<^bold>p\<^bold>r\<^bold>e\<^bold>m\<^bold>i\<^bold>s\<^bold>e P x \<longrightarrow> \<^bold>p\<^bold>r\<^bold>o\<^bold>c body \<blangle> X x \<longmapsto> \<exists>* x'. X x' \<heavy_comma>^ P x' \<tycolon> \<bool> \<brangle>)
   \<longrightarrow> \<^bold>p\<^bold>r\<^bold>e\<^bold>m\<^bold>i\<^bold>s\<^bold>e P x \<longrightarrow> \<^bold>p\<^bold>r\<^bold>o\<^bold>c DoWhile body \<blangle> X x \<longmapsto> \<exists>* x'. X x' \<and>\<^sup>s (\<not> P x') \<brangle>"
 (*  for X :: "(heap \<times> 'a::lrep, 'b) \<nu>" *)
   unfolding DoWhile_def Procedure_def Auto_def
-  apply (auto simp add: SemDoWhile_deterministic2 simp add: nu_exps)
-  subgoal for a b xa
+  apply (auto simp add: SemDoWhile_deterministic2 nu_exps Heap'_Stack_Front Heap'_ExSet Heap'_Addition)
+  subgoal for a b xa H
     apply (rotate_tac 2)
     by (induct  body "(a, b)" xa arbitrary: a b x rule: SemDoWhile.induct) (auto 0 7 simp add: nu_exps)
   done
+declare Heap'_expn[simp]
 
 
 lemma do_while_\<nu>app:
@@ -228,6 +230,7 @@ lemma SemRec_deterministic2: " SemRec body s x \<Longrightarrow> The ( SemRec bo
 definition op_recursion :: "(('x \<longmapsto> 'y) \<Rightarrow> ('x \<longmapsto> 'y)) \<Rightarrow> 'x \<longmapsto> 'y"
   where "op_recursion F s = (if (\<exists>t. SemRec F s t) then The (SemRec F s) else PartialCorrect)"
 
+declare Heap'_expn[simp del]
 lemma op_recursion:
   "(\<And>g x'. (\<forall>x''. \<^bold>f\<^bold>u\<^bold>n\<^bold>c g \<blangle> X x'' \<longmapsto> Y x'' \<brangle>) \<longrightarrow> \<^bold>f\<^bold>u\<^bold>n\<^bold>c F g \<blangle> X x' \<longmapsto> Y x' \<brangle>) \<Longrightarrow>
     (\<forall>x. \<^bold>f\<^bold>u\<^bold>n\<^bold>c op_recursion F \<blangle> X x \<longmapsto> Y x \<brangle>)"
@@ -235,6 +238,7 @@ lemma op_recursion:
   unfolding op_recursion_def Procedure_def Function_def atomize_all
   apply (auto simp add: SemRec_deterministic2)
   subgoal for x a b xa apply (rotate_tac 1) apply (induct rule:  SemRec.induct) by (auto 0 6) done
+declare Heap'_expn[simp]
 
 section \<open>Arithmetic instructions\<close>
 
@@ -254,28 +258,32 @@ theorem const_nat_\<nu>app: "\<^bold>p\<^bold>r\<^bold>o\<^bold>c op_const_int T
 lemma [\<nu>intro]:
   "\<^bold>p\<^bold>r\<^bold>e\<^bold>m\<^bold>i\<^bold>s\<^bold>e (numeral x :: nat) < 2^LENGTH('w) \<Longrightarrow>
    \<^bold>c\<^bold>o\<^bold>n\<^bold>s\<^bold>t\<^bold>r\<^bold>u\<^bold>c\<^bold>t ((numeral x) \<tycolon> \<nat>['w]) \<^bold>b\<^bold>y \<^bold>p\<^bold>r\<^bold>o\<^bold>c op_const_int TYPE('w::len) (Word.of_nat (numeral x))
-    \<blangle> R\<heavy_comma> \<^bold>h\<^bold>e\<^bold>a\<^bold>p Nothing \<longmapsto> R \<heavy_comma> (numeral x) \<tycolon> \<nat>['w]\<heavy_comma> \<^bold>h\<^bold>e\<^bold>a\<^bold>p Nothing \<brangle>"
+    \<blangle> R\<heavy_comma> \<^bold>h\<^bold>e\<^bold>a\<^bold>p H \<longmapsto> R \<heavy_comma> (numeral x) \<tycolon> \<nat>['w]\<heavy_comma> \<^bold>h\<^bold>e\<^bold>a\<^bold>p H \<brangle>"
   unfolding op_const_int_def \<nu>def including show_more1 by (auto simp add: nu_exps) (metis mod_if unat_bintrunc unat_numeral)
   \<comment> \<open>Only literal number could be constructed automatically\<close>
+
 lemma [\<nu>intro]:
   "\<^bold>c\<^bold>o\<^bold>n\<^bold>s\<^bold>t\<^bold>r\<^bold>u\<^bold>c\<^bold>t (0 \<tycolon> \<nat>['w]) \<^bold>b\<^bold>y \<^bold>p\<^bold>r\<^bold>o\<^bold>c op_const_int TYPE('w::len) 0
-    \<blangle> R\<heavy_comma> \<^bold>h\<^bold>e\<^bold>a\<^bold>p Nothing \<longmapsto> R \<heavy_comma> 0 \<tycolon> \<nat>['w]\<heavy_comma> \<^bold>h\<^bold>e\<^bold>a\<^bold>p Nothing \<brangle>"
-  unfolding AutoConstruct_def using const_nat_\<nu>app by (metis unat_0) 
+    \<blangle> R\<heavy_comma> \<^bold>h\<^bold>e\<^bold>a\<^bold>p H \<longmapsto> R \<heavy_comma> 0 \<tycolon> \<nat>['w]\<heavy_comma> \<^bold>h\<^bold>e\<^bold>a\<^bold>p H \<brangle>"
+  unfolding AutoConstruct_def \<nu>def op_const_int_def by (auto simp add: nu_exps)
+
 lemma [\<nu>intro]:
   "\<^bold>c\<^bold>o\<^bold>n\<^bold>s\<^bold>t\<^bold>r\<^bold>u\<^bold>c\<^bold>t (1 \<tycolon> \<nat>['w]) \<^bold>b\<^bold>y \<^bold>p\<^bold>r\<^bold>o\<^bold>c op_const_int TYPE('w::len) 1
-    \<blangle> R\<heavy_comma> \<^bold>h\<^bold>e\<^bold>a\<^bold>p Nothing \<longmapsto> R\<heavy_comma> 1 \<tycolon> \<nat>['w]\<heavy_comma> \<^bold>h\<^bold>e\<^bold>a\<^bold>p Nothing \<brangle>"
-  unfolding AutoConstruct_def using const_nat_\<nu>app by (metis unat_1)
+    \<blangle> R\<heavy_comma> \<^bold>h\<^bold>e\<^bold>a\<^bold>p H \<longmapsto> R\<heavy_comma> 1 \<tycolon> \<nat>['w]\<heavy_comma> \<^bold>h\<^bold>e\<^bold>a\<^bold>p H \<brangle>"
+  unfolding AutoConstruct_def \<nu>def op_const_int_def by (auto simp add: nu_exps)
 
 lemma [\<nu>intro]:
   "\<^bold>p\<^bold>r\<^bold>e\<^bold>m\<^bold>i\<^bold>s\<^bold>e (numeral x :: nat) < 2^LENGTH('w) \<Longrightarrow>
    \<^bold>c\<^bold>o\<^bold>n\<^bold>s\<^bold>t\<^bold>r\<^bold>u\<^bold>c\<^bold>t ((numeral x) \<tycolon> \<nat>\<^sup>r['w]) \<^bold>b\<^bold>y \<^bold>p\<^bold>r\<^bold>o\<^bold>c op_const_int TYPE('w::len) (Word.of_nat (numeral x))
-    \<blangle> R\<heavy_comma> \<^bold>h\<^bold>e\<^bold>a\<^bold>p Nothing \<longmapsto> R\<heavy_comma> (numeral x) \<tycolon> \<nat>\<^sup>r['w]\<heavy_comma> \<^bold>h\<^bold>e\<^bold>a\<^bold>p Nothing \<brangle>"
+    \<blangle> R\<heavy_comma> \<^bold>h\<^bold>e\<^bold>a\<^bold>p H \<longmapsto> R\<heavy_comma> (numeral x) \<tycolon> \<nat>\<^sup>r['w]\<heavy_comma> \<^bold>h\<^bold>e\<^bold>a\<^bold>p H \<brangle>"
   unfolding op_const_int_def \<nu>def including show_more1 by (auto simp add: nu_exps)
+
 lemma [\<nu>intro]:
-  "\<^bold>c\<^bold>o\<^bold>n\<^bold>s\<^bold>t\<^bold>r\<^bold>u\<^bold>c\<^bold>t (0 \<tycolon> \<nat>\<^sup>r['w]) \<^bold>b\<^bold>y \<^bold>p\<^bold>r\<^bold>o\<^bold>c op_const_int TYPE('w::len) 0 \<blangle> R\<heavy_comma> \<^bold>h\<^bold>e\<^bold>a\<^bold>p Nothing \<longmapsto> R\<heavy_comma> 0 \<tycolon> \<nat>\<^sup>r['w]\<heavy_comma> \<^bold>h\<^bold>e\<^bold>a\<^bold>p Nothing \<brangle>"
+  "\<^bold>c\<^bold>o\<^bold>n\<^bold>s\<^bold>t\<^bold>r\<^bold>u\<^bold>c\<^bold>t (0 \<tycolon> \<nat>\<^sup>r['w]) \<^bold>b\<^bold>y \<^bold>p\<^bold>r\<^bold>o\<^bold>c op_const_int TYPE('w::len) 0 \<blangle> R\<heavy_comma> \<^bold>h\<^bold>e\<^bold>a\<^bold>p H \<longmapsto> R\<heavy_comma> 0 \<tycolon> \<nat>\<^sup>r['w]\<heavy_comma> \<^bold>h\<^bold>e\<^bold>a\<^bold>p H \<brangle>"
   unfolding op_const_int_def \<nu>def including show_more1 by (auto simp add: nu_exps)
+
 lemma [\<nu>intro]:
-  "\<^bold>c\<^bold>o\<^bold>n\<^bold>s\<^bold>t\<^bold>r\<^bold>u\<^bold>c\<^bold>t (1 \<tycolon> \<nat>\<^sup>r['w]) \<^bold>b\<^bold>y \<^bold>p\<^bold>r\<^bold>o\<^bold>c op_const_int TYPE('w::len) 1 \<blangle> R\<heavy_comma> \<^bold>h\<^bold>e\<^bold>a\<^bold>p Nothing \<longmapsto> R\<heavy_comma> 1 \<tycolon> \<nat>\<^sup>r['w]\<heavy_comma> \<^bold>h\<^bold>e\<^bold>a\<^bold>p Nothing \<brangle>"
+  "\<^bold>c\<^bold>o\<^bold>n\<^bold>s\<^bold>t\<^bold>r\<^bold>u\<^bold>c\<^bold>t (1 \<tycolon> \<nat>\<^sup>r['w]) \<^bold>b\<^bold>y \<^bold>p\<^bold>r\<^bold>o\<^bold>c op_const_int TYPE('w::len) 1 \<blangle> R\<heavy_comma> \<^bold>h\<^bold>e\<^bold>a\<^bold>p H \<longmapsto> R\<heavy_comma> 1 \<tycolon> \<nat>\<^sup>r['w]\<heavy_comma> \<^bold>h\<^bold>e\<^bold>a\<^bold>p H \<brangle>"
   unfolding op_const_int_def \<nu>def including show_more1 by (auto simp add: nu_exps)
 
 (* schematic_goal "\<^bold>c\<^bold>o\<^bold>n\<^bold>s\<^bold>t\<^bold>r\<^bold>u\<^bold>c\<^bold>t 3 \<^bold>b\<^bold>y \<^bold>p\<^bold>r\<^bold>o\<^bold>c ?f
@@ -518,7 +526,7 @@ definition op_load :: " llty \<Rightarrow> ('a::lrep,'a,'ax,'ax) index \<Rightar
       if lty = LLTY('a) then Success (heap, get_idx idx (shallowize data), r) else Fail
     | _ \<Rightarrow> Fail))"
 
-theorem op_load[ \<nu>overload "\<up>:" ]:
+lemma op_load[ \<nu>overload "\<up>:" ]:
   "FieldIndex field_index Y X gt mp \<longrightarrow>
   \<^bold>p\<^bold>r\<^bold>o\<^bold>c op_load LLTY('x) field_index \<blangle> R\<heavy_comma> addr \<tycolon> Pointer\<heavy_comma> \<^bold>h\<^bold>e\<^bold>a\<^bold>p H \<heavy_asterisk> addr \<R_arr_tail> x \<tycolon> Ref X \<longmapsto> R\<heavy_comma> gt x \<tycolon> Y\<heavy_comma> \<^bold>h\<^bold>e\<^bold>a\<^bold>p H \<heavy_asterisk> addr \<R_arr_tail> x \<tycolon> Ref X\<brangle> "
   for X :: "('x::field, 'c) \<nu>"
@@ -546,7 +554,7 @@ definition op_store :: " llty \<Rightarrow> ('a::lrep,'a,'ax,'ax) index \<Righta
       if lty = LLTY('a) then Success (heap(key \<mapsto> map_deepmodel (map_idx idx (\<lambda>_. x)) data), memptr addr, r) else Fail
     | _ \<Rightarrow> Fail))"
 
-theorem op_store[ \<nu>overload "\<down>:" ]:
+lemma op_store[ \<nu>overload "\<down>:" ]:
   "FieldIndex field_index Y X gt mp \<longrightarrow>
   \<^bold>p\<^bold>r\<^bold>o\<^bold>c op_store LLTY('x) field_index
     \<blangle> R\<heavy_comma> addr \<tycolon> Pointer\<heavy_comma> y \<tycolon> Y\<heavy_comma> \<^bold>h\<^bold>e\<^bold>a\<^bold>p addr \<R_arr_tail> x \<tycolon> Ref X \<longmapsto> R \<heavy_comma> addr \<tycolon> Pointer \<heavy_comma> \<^bold>h\<^bold>e\<^bold>a\<^bold>p addr \<R_arr_tail> mp (\<lambda>_. y) x \<tycolon> Ref X\<brangle> "
@@ -569,16 +577,20 @@ proc i_store_n[\<nu>overload "\<down>:"]:
   \<open>R\<heavy_comma> a \<tycolon> Pointer\<heavy_comma> i \<tycolon> \<nat>[size_t]\<heavy_comma> y \<tycolon> Y \<heavy_comma> \<^bold>h\<^bold>e\<^bold>a\<^bold>p a \<R_arr_tail> xs \<tycolon> Array X\<close> \<longmapsto> \<open>R\<heavy_comma> \<^bold>h\<^bold>e\<^bold>a\<^bold>p a \<R_arr_tail> xs[i := mp (\<lambda>_. y) (xs ! i)] \<tycolon> Array X\<close>
   for Y :: "('y::field, 'd) \<nu>"
   requires [used]: "\<^bold>p\<^bold>r\<^bold>e\<^bold>m\<^bold>i\<^bold>s\<^bold>e i < length xs" and idx: "FieldIndex field_index Y X gt mp"
-  \<bullet> \<rightarrow> y
-  \<bullet> + y
-  \<bullet> \<down>: idx drop
+  \<bullet> \<rightarrow> y + y \<down>: idx drop
   finish
 
 lemmas [ \<nu>overload "\<down>" ] = i_store_n_\<nu>app[THEN mp, THEN mp, OF _ FieldIndex_here, unfolded atomize_imp, simplified]
 
+declare Nat.One_nat_def[simp del] Num.add_2_eq_Suc'[simp] split_paired_All[simp]
+
+bundle xx = Nat.One_nat_def[simp del] Num.add_2_eq_Suc'[simp] split_paired_All[simp]
 
 fun fib where
   "fib 0 = 1" | "fib (Suc 0) = 1" | "fib (Suc (Suc n)) = fib n + fib (Suc n)"
+lemma [simp]: "fib 1 = 1" by (simp add: One_nat_def) 
+lemma [simp]: "fib (j + 1 + 1) = fib j + fib (j + 1)"
+  by (metis Suc_eq_plus1 fib.simps(3))
 
 (* int fib (int i) { if (i \<le> 1) return 1; else return fib (i-2) + fib (i-1); } *)
 rec_proc Fib: \<open>i \<tycolon> \<nat>[32]\<close> \<longmapsto> \<open>fib i \<tycolon> \<nat>\<^sup>r[32]\<close> var i
@@ -586,5 +598,13 @@ rec_proc Fib: \<open>i \<tycolon> \<nat>[32]\<close> \<longmapsto> \<open>fib i 
   \<bullet> cast ie \<open>fib i\<close> affirm by (cases i rule: fib.cases) auto
   finish
 
+proc Fib2: \<open>i \<tycolon> \<nat>[32]\<close> \<longmapsto> \<open>fib i \<tycolon> \<nat>\<^sup>r[32]\<close>
+  \<bullet> \<rightarrow> i \<open>1\<tycolon> \<nat>\<^sup>r[32]\<close> 1 \<open>0 \<tycolon> \<nat>[32]\<close>
+  \<bullet> while var fj_1 fj j in fj, fj_1, j always \<open>fj = fib j \<and> fj_1 = fib (j + 1) \<and> j \<le> i\<close>
+  \<bullet> \<medium_left_bracket> dup i < \<medium_right_bracket>
+  \<bullet> \<medium_left_bracket> \<rightarrow> fj, fj_1, j fj_1 fj fj_1 + j 1 + \<medium_right_bracket>
+  have [simp]: "j = i \<and> fj = fib i" using \<glowing_star> by auto
+  \<bullet> drop^2
+  finish
 
 end
